mppa_k1c/Asmblockgenproof1.v
@@ -2110,6 +2110,26 @@ Proof.
   inv EV. repeat eexists. eassumption. econstructor; eauto.
 Qed.
 
+Lemma transl_memory_access2XS_correct:
+  forall chunk mk_instr (scale : Z) args k c (rs: regset) m v,
+  transl_memory_access2XS chunk mk_instr scale args k = OK c ->
+  eval_addressing ge rs#SP (Aindexed2XS scale) (map rs (map preg_of args)) = Some v ->
+  exists base ro mro mr1 rs',
+     args = mr1 :: mro :: nil
+  /\ ireg_of mro = OK ro
+  /\ exec_straight_opt (basics_to_code c) rs m (mk_instr base ro ::g (basics_to_code k)) rs' m
+  /\ Val.addl rs'#base (Val.shll rs'#ro (Vint (Int.repr scale))) = v
+  /\ (forall r, r <> PC -> r <> RTMP -> rs'#r = rs#r)
+  /\ scale = (zscale_of_chunk chunk).
+Proof.
+  intros until v; intros TR EV. 
+  unfold transl_memory_access2XS in TR; ArgsInv.
+  inv EV. repeat eexists. eassumption. econstructor; eauto.
+  symmetry.
+  apply Z.eqb_eq.
+  assumption.
+Qed.
+
 Lemma transl_load_access2_correct:
   forall chunk (mk_instr: ireg -> ireg -> basic) addr args k c rd (rs: regset) m v mro mr1 ro v',
   args = mr1 :: mro :: nil ->
@@ -2130,6 +2150,32 @@ Proof.
   econstructor; split.
   eapply exec_straight_opt_right. eexact A. apply exec_straight_one. assert (ro = ro2) by congruence. subst ro2.
   rewrite INSTR. unfold exec_load_reg. unfold parexec_load_reg. rewrite B, LOAD. reflexivity. Simpl. 
+  split; intros; Simpl. auto.
+Qed.
+
+Lemma transl_load_access2XS_correct:
+  forall chunk (mk_instr: ireg -> ireg -> basic) (scale : Z) args k c rd (rs: regset) m v mro mr1 ro v',
+  args = mr1 :: mro :: nil ->
+  ireg_of mro = OK ro ->
+  (forall base rs,
+     exec_basic_instr ge (mk_instr base ro) rs m = exec_load_regxs chunk rs m rd base ro) ->
+  transl_memory_access2XS chunk mk_instr scale args k = OK c ->
+  eval_addressing ge rs#SP (Aindexed2XS scale) (map rs (map preg_of args)) = Some v ->
+  Mem.loadv chunk m v = Some v' ->
+  exists rs',
+     exec_straight ge (basics_to_code c) rs m (basics_to_code k) rs' m
+  /\ rs'#rd = v'
+  /\ forall r, r <> PC -> r <> RTMP -> r <> rd -> rs'#r = rs#r.
+Proof.
+  intros until v'; intros ARGS IREGE INSTR TR EV LOAD. 
+  exploit transl_memory_access2XS_correct; eauto.
+  intros (base & ro2 & mro2 & mr2 & rs' & ARGSS & IREGEQ & A & B & C & D). rewrite ARGSS in ARGS. inversion ARGS. subst mr2 mro2. clear ARGS.
+  econstructor; split.
+  eapply exec_straight_opt_right. eexact A. apply exec_straight_one. assert (ro = ro2) by congruence. subst ro2.
+  rewrite INSTR. unfold exec_load_regxs. unfold parexec_load_regxs.
+  unfold scale_of_chunk.
+  subst scale.
+  rewrite B, LOAD. reflexivity. Simpl. 
   split; intros; Simpl. auto.
 Qed.
 
@@ -2168,7 +2214,6 @@ Lemma transl_load_memory_access_ok:
 Proof.
   intros until m. intros ADDR TR ? ?.
   unfold transl_load in TR. destruct addr; try contradiction.
-  - admit.
   - monadInv TR. destruct chunk; ArgsInv; econstructor; (esplit; eauto).
   - monadInv TR. destruct chunk. all: ArgsInv; destruct args; try discriminate; monadInv EQ0; eexists; eexists; split; try split;
     [ instantiate (1 := (PLoadRRO _ x)); simpl; reflexivity
@@ -2200,6 +2245,27 @@ Proof.
   | eauto].
 Qed.
 
+Lemma transl_load_memory_access2XS_ok:
+  forall scale chunk args dst k c rs a v m,
+  transl_load chunk (Aindexed2XS scale) args dst k = OK c ->
+  eval_addressing ge (rs (IR SP)) (Aindexed2XS scale) (map rs (map preg_of args)) = Some a ->
+  Mem.loadv chunk m a = Some v ->
+  exists mk_instr mr0 mro rd ro,
+      args = mr0 :: mro :: nil
+   /\ preg_of dst = IR rd
+   /\ preg_of mro = IR ro
+   /\ transl_memory_access2XS chunk mk_instr (Aindexed2XS scale) args k = OK c
+   /\ forall base rs,
+      exec_basic_instr ge (mk_instr base ro) rs m = exec_load_reg chunk rs m rd base ro.
+Proof.
+  intros until m. intros TR ? ?.
+  unfold transl_load in TR. subst. monadInv TR. destruct chunk. all:
+  unfold transl_memory_access2XS in EQ0; repeat (destruct args; try discriminate); monadInv EQ0; ArgsInv; repeat eexists;
+  [ unfold ireg_of in EQ0; destruct (preg_of m1); eauto; try discriminate; monadInv EQ0; reflexivity
+  | rewrite EQ1; rewrite EQ0; simpl; instantiate (1 := (PLoadRRR _ x)); simpl; rewrite Heqb; reflexivity
+  | eauto].
+Qed.
+
 Lemma transl_load_correct:
   forall chunk addr args dst k c (rs: regset) m a v,
   transl_load chunk addr args dst k = OK c ->
@@ -2211,12 +2277,19 @@ Lemma transl_load_correct:
   /\ forall r, r <> PC -> r <> RTMP -> r <> preg_of dst -> rs'#r = rs#r.
 Proof.
   intros until v; intros TR EV LOAD. destruct addr.
-  1: (* Aindexed2XS *) discriminate.
-  2-4: exploit transl_load_memory_access_ok; eauto; try discriminate;
-    intros A; destruct A as (mk_instr & rd & rdEq & B & C); rewrite rdEq;
-    eapply transl_load_access_correct; eauto with asmgen.
+  - exploit transl_load_memory_access2XS_ok; eauto. intros (mk_instr & mr0 & mro & rd & ro & argsEq & rdEq & roEq & B & C).
+    rewrite rdEq. eapply transl_load_access2XS_correct; eauto with asmgen. unfold ireg_of. rewrite roEq. reflexivity.
   - exploit transl_load_memory_access2_ok; eauto. intros (mk_instr & mr0 & mro & rd & ro & argsEq & rdEq & roEq & B & C).
     rewrite rdEq. eapply transl_load_access2_correct; eauto with asmgen. unfold ireg_of. rewrite roEq. reflexivity.
+  - exploit transl_load_memory_access_ok; eauto; try discriminate; try (simpl; reflexivity).
+    intros A; destruct A as (mk_instr & rd & rdEq & B & C); rewrite rdEq;
+      eapply transl_load_access_correct; eauto with asmgen.
+  - exploit transl_load_memory_access_ok; eauto; try discriminate; try (simpl; reflexivity).
+    intros A; destruct A as (mk_instr & rd & rdEq & B & C); rewrite rdEq;
+      eapply transl_load_access_correct; eauto with asmgen.
+  - exploit transl_load_memory_access_ok; eauto; try discriminate; try (simpl; reflexivity).
+    intros A; destruct A as (mk_instr & rd & rdEq & B & C); rewrite rdEq;
+      eapply transl_load_access_correct; eauto with asmgen.
 Qed.
 
 Lemma transl_store_access2_correct:
